exercises/project01-distributed-lock-server/host.v.dfy
@@ -13,23 +13,14 @@ module Host {
 
   // Define your Message datatype here.
   datatype Message =
-    //#solution
     Grant(dest:HostId, epoch:nat)
-    //#stub
-    // Message() // Populate this datatype.
-    //#end
 
   // Define your Host protocol state machine here.
   datatype Constants = Constants(numHosts: nat, myId:HostId)
 
   datatype Variables = Variables(
-    //#solution
     c: Constants,
     holdsLock:bool, epoch:nat
-    //#stub
-    // c: Constants
-    //// Fill me in.
-    //#end
   )
 
   // You can assume in Init below that the initial constants are set by the
@@ -37,56 +28,40 @@ module Host {
   // machine knows the correct total number of hosts and its own ID.
 
   ghost predicate Init(v:Variables) {
-    //#solution
     && v.holdsLock == (v.c.myId == 0)
     && v.epoch == if v.c.myId == 0 then 1 else 0
-       //#stub
-       // true // Replace me
-       //#end
   }
-  //#solution
-  ghost predicate DoGrant(v:Variables, v':Variables, msgOps:Network.MessageOps<Message>, step: Step)
-    requires step.DoGrantStep?
+
+  ghost predicate DoGrant(v:Variables, v':Variables, msgOps:Network.MessageOps<Message>, recipient:HostId)
   {
-    var recipient := step.recipient;
-    && v.holdsLock == true
     && msgOps.recv.None?
-    && ValidHostId(v.c.numHosts, recipient) // Doesn't actually affect safety, but does affect liveness! if we grant to msgOps nonexistent host, no further steps will occur.
+    && v.holdsLock == true
+    && ValidHostId(v.c.numHosts, recipient)
     && msgOps.send == Some(Grant(recipient, v.epoch + 1))
     && v'.holdsLock == false
     && v'.epoch == v.epoch
   }
 
-  ghost predicate DoAccept(v:Variables, v':Variables, msgOps:Network.MessageOps<Message>, step: Step)
-    requires step.DoAcceptStep?
+  ghost predicate DoAccept(v:Variables, v':Variables, msgOps:Network.MessageOps<Message>)
   {
     && msgOps.recv.Some?
     && msgOps.recv.value.dest == v.c.myId
     && msgOps.recv.value.epoch > v.epoch
-    && msgOps.send == None
-    && v'.epoch == msgOps.recv.value.epoch
+    && msgOps.send.None?
     && v'.holdsLock == true
+    && v'.epoch == msgOps.recv.value.epoch
   }
-  //#stub
-  //#end
+
   // JayNF
   datatype Step =
-      //#solution
     | DoGrantStep(recipient: HostId)
     | DoAcceptStep
-      //#stub
-    // | SomeStep   // Replace me
-    //#end
 
   ghost predicate NextStep(v:Variables, v':Variables, msgOps:Network.MessageOps<Message>, step: Step) {
     && v'.c == v.c
     && match step
-       //#solution
-       case DoGrantStep(_) => DoGrant(v, v', msgOps, step)
-       case DoAcceptStep => DoAccept(v, v', msgOps, step)
-       //#stub
-       // case SomeStep => true
-       //#end
+       case DoGrantStep(recipient) => DoGrant(v, v', msgOps, recipient)
+       case DoAcceptStep => DoAccept(v, v', msgOps)
   }
 
   lemma NextStepDeterministic(v: Variables, v'1: Variables, v'2: Variables, msgOps: Network.MessageOps<Message>, step: Step)
